BTree_Imp.thy
@@ -1,0 +1,71 @@
+theory BTree_Imp
+  imports "Separation_Logic_Imperative_HOL.Sep_Main"
+begin
+
+datatype 'a btree = Leaf | Node "('a btree * 'a) list" "'a btree"
+
+datatype 'a btnode = Btnode "('a btnode ref option*'a) array" "'a
+btnode ref option"
+
+text \<open>Encoding to natural numbers, as required by Imperative/HOL\<close>
+(* Sollte auch mit deriving gehen *)
+fun
+  btnode_encode :: "'a::heap btnode \<Rightarrow> nat"
+where
+  "btnode_encode (Btnode ts t) = to_nat (ts, t)"
+
+instance btnode :: (heap) heap
+  apply (rule heap_class.intro)
+  apply (rule countable_classI [of "btnode_encode"])
+  apply (metis btnode_encode.elims from_nat_to_nat fst_conv snd_conv)
+  ..
+
+  
+context fixes A :: "'a \<Rightarrow> 'b \<Rightarrow> assn"
+begin
+  fun list_assn where
+    "list_assn [] [] = emp"
+  | "list_assn (x#xs) (y#ys) = A x y * list_assn xs ys"  
+  | "list_assn _ _ = false"
+end
+
+
+lemma list_assn_cong[fundef_cong]:
+  "\<lbrakk> xs=xs'; ys=ys'; \<And>x y. \<lbrakk> x\<in>set xs; y\<in>set ys \<rbrakk> \<Longrightarrow> A x y = A' x y \<rbrakk> \<Longrightarrow>
+list_assn A xs ys = list_assn A' xs' ys'"
+  apply (induction xs ys arbitrary: xs' ys' rule: list_assn.induct)
+  apply auto
+  done
+  
+thm map_cong
+
+
+
+fun prod_assn (infixr "\<times>\<^sub>a" 80) where
+  "prod_assn A B (a,b) (ai,bi) = A a ai * B b bi"
+
+  
+lemma prod_assn_cong[fundef_cong]:
+  "\<lbrakk> p=p'; pi=pi'; A (fst p) (fst pi) = A' (fst p) (fst pi); B (snd p)
+(snd pi) = B' (snd p) (snd pi) \<rbrakk> 
+    \<Longrightarrow> (A\<times>\<^sub>aB) p pi = (A'\<times>\<^sub>aB') p' pi'" 
+    apply (cases p; cases pi)
+    by auto
+  
+  
+abbreviation "id_assn x y \<equiv> \<up>(x=y)"
+
+    
+fun R where
+"R None Leaf = emp" |
+"R (Some a) (Node ts t) = 
+ (\<exists>\<^sub>A tsi ti xsi. 
+      a \<mapsto>\<^sub>r Btnode tsi ti 
+    * R ti t 
+    * tsi \<mapsto>\<^sub>a xsi
+    * list_assn (R \<times>\<^sub>a id_assn) xsi ts
+    )" |
+"R _ _ = false"
+
+
+end
